src/UpdList.v
@@ -1,0 +1,74 @@
+Require Import Automation.
+Require Import Mem.
+
+Require Import List.
+Import ListNotations.
+Open Scope list_scope.
+
+Set Implicit Arguments.
+
+Fixpoint upd_all AT AEQ V (m: @mem AT AEQ V) (l: list (AT*V)) :=
+  match l with
+  | nil => m
+  | (a,v)::l' => upd (upd_all m l') a v
+  end.
+
+Lemma upd_all_incr_domain : forall AT AEQ V (m:@mem AT AEQ V) a ws,
+    (exists v, m a = Some v) ->
+    (exists v, upd_all m ws a = Some v).
+Proof.
+  induction ws; intros; simpl; repeat deex; eauto.
+  destruct a0.
+  destruct (AEQ a a0); subst; autorewrite with upd; eauto.
+Qed.
+
+Theorem upd_all_nodup_in : forall AT AEQ V (m:@mem AT AEQ V) ws a v,
+    NoDup (map fst ws) ->
+    In (a, v) ws ->
+    upd_all m ws a = Some v.
+Proof.
+  induction ws; simpl; intros.
+  contradiction.
+
+  destruct a as [a' v'].
+  simpl in *.
+  inversion H; subst.
+  intuition eauto.
+  inversion H1; subst;
+    autorewrite with upd; auto.
+  destruct (AEQ a' a0); subst;
+    autorewrite with upd;
+    eauto.
+  contradict H3.
+  change a0 with (fst (a0, v)).
+  auto using in_map.
+Qed.
+
+Theorem upd_all_not_in : forall AT AEQ V (m:@mem AT AEQ V) ws a,
+    ~List.In a (List.map fst ws) ->
+    upd_all m ws a = m a.
+Proof.
+  induction ws; simpl; intros; eauto.
+  destruct a as [a' v]; simpl in *.
+  intuition eauto.
+  autorewrite with upd; eauto.
+Qed.
+
+Lemma list_addr_in_dec : forall A B (AEQ:forall (a a':A), {a=a'}+{a<>a'})
+                           a (l: list (A * B)),
+    {v | List.In (a, v) l} + {~List.In a (List.map fst l)}.
+Proof.
+  intros.
+  destruct (List.In_dec AEQ a (List.map fst l)); eauto.
+  left.
+  induction l; simpl in *.
+  contradiction.
+  destruct a0 as [a' v]; simpl in *.
+  destruct (AEQ a a'); subst; eauto.
+  destruct IHl; eauto.
+  intuition congruence.
+Defined.
+
+(* upd_all_nodup_in requires erewrite for the value, so it can't be added as a
+rewrite hint. *)
+Hint Rewrite upd_all_not_in using solve [ auto ] : upd.
